Header getter specs

src/c/include/coq-vsu-certicoq-block/block.h
@@ -17,17 +17,18 @@ certicoq_block_header_t *certicoq_block__get_header_ptr(const certicoq_block_t b
 void certicoq_block__set_header(certicoq_block_t block, const certicoq_block_header_t *header);
 
 size_t certicoq_block__get_size(const certicoq_block_header_t *header);
+
 size_t certicoq_block__get_field_count(const certicoq_block_header_t *header);
 void certicoq_block__set_field_count(certicoq_block_header_t *header, size_t size);
 
 certicoq_block_tag_t certicoq_block__get_tag(const certicoq_block_header_t *header);
 certicoq_block_header_t certicoq_block__set_tag(certicoq_block_header_t *header, certicoq_block_tag_t tag);
 
+uint8_t certicoq_block__get_odata(const certicoq_block_header_t *header);
+void certicoq_block__set_odata(certicoq_block_header_t *header, uint8_t odata);
+
 int_or_ptr *certicoq_block__get_field_ptr(certicoq_block_t block, size_t field);
 int_or_ptr certicoq_block__get_field(const certicoq_block_t block, size_t field);
 void certicoq_block__set_field(certicoq_block_t block, size_t field, int_or_ptr x);
-
-uintptr_t certicoq_block__get_odata(const certicoq_block_t block);
-void certicoq_block__set_odata(certicoq_block_t block, uintptr_t odata);
 
 #endif /* COQ_CERTICOQ_BLOCK__BLOCK_H */
