src/c/include/coq-vsu-certicoq-block/src/block.c
@@ -41,27 +41,41 @@ void certicoq_block__set_header(certicoq_block_t block, const certicoq_block_hea
 
 size_t certicoq_block__get_size(const certicoq_block_header_t *header)
 {
-    return 1 + certicoq_block__get_field_count(header);
+    const size_t zero = 0;
+    const size_t one = 1;
+    const size_t two = 2;
+    const size_t fc = certicoq_block__get_field_count(header);
+    return fc > zero ? one + fc : two;
 }
 
 size_t certicoq_block__get_field_count(const certicoq_block_header_t *header)
 {
-    return (*header) >> 10;
+    return (header[0]) >> 10;
 }
 
 void certicoq_block__set_field_count(certicoq_block_header_t *header, size_t size)
 {
-    *header = ((*header) & ~((1 << 10) - 1)) | (size << 10);
+    header[0] = ((header[0]) & ~((1 << 10) - 1)) | (size << 10);
 }
 
 certicoq_block_tag_t certicoq_block__get_tag(const certicoq_block_header_t *header)
 {
-    return (*header) & 0xff;
+    return (header[0]) & 0xff;
 }
 
 certicoq_block_header_t certicoq_block__set_tag(certicoq_block_header_t *header, certicoq_block_tag_t tag)
 {
-    return ((*header) & ~0xff) | tag;
+    return ((header[0]) & ~0xff) | tag;
+}
+
+uint8_t certicoq_block__get_odata(const certicoq_block_header_t *header)
+{
+    return (header[0] >> 8) & 0x03;
+}
+
+void certicoq_block__set_odata(certicoq_block_header_t *header, uint8_t odata)
+{
+    header[0] = (header[0] & ~(0x03 << 8)) | (odata << 8);
 }
 
 int_or_ptr *certicoq_block__get_field_ptr(certicoq_block_t block, size_t field)
@@ -77,16 +91,6 @@ int_or_ptr certicoq_block__get_field(const certicoq_block_t block, size_t field)
 void certicoq_block__set_field(certicoq_block_t block, size_t field, int_or_ptr x)
 {
     block[field] = x;
-}
-
-uintptr_t certicoq_block__get_odata(const certicoq_block_t block)
-{
-    return 0; // TODO
-}
-
-void certicoq_block__set_odata(certicoq_block_t block, uintptr_t odata)
-{
-    // TODO
 }
 
 #endif /* COQ_CERTICOQ_BLOCK__BLOCK_H */
