theories/Block/vst/cmodel/certicoq_block.v
@@ -1,25 +1,55 @@
+From Coq Require Import micromega.Lia.
 From Coq Require Import ZArith.ZArith.
-
-From compcert Require Import common.Values.
-From compcert Require Import lib.Integers.
-
-From VST Require Import floyd.sublist.
-From VST Require Import veric.val_lemmas.
 
 From appliedfm Require Import int_or_ptr.vst.cmodel.constants.
 From appliedfm Require Import int_or_ptr.vst.cmodel.val.
 
+From CertiCoq Require Import Block.vst.cmodel.certicoq_block_header.
 
-Record header :=
-{
-  header_tag: Z;
-  header_size: Z;
-  header_tag__range: (0 <= header_tag < 256)%Z;
-}.
+Local Open Scope Z.
 
-Record block (odata: Type) := {
-    block_header: header;
-    block_odata: odata;
+Record Block := {
+    block_header:> BlockHeader;
     block_fields: list int_or_ptr;
-    block_fields__range: (0 < Zlength block_fields < two_p (word_size * 8 - 10))%Z;
+    block_fields__block_header_field_count: Zlength block_fields = block_header_field_count block_header;
 }.
+
+Lemma block_fields__Zlength (b: Block):
+    0 <= Zlength (block_fields b) < two_p (word_size * 8 - 10).
+Proof.
+    rewrite block_fields__block_header_field_count.
+    apply block_header_field_count__range.
+Qed.
+
+Definition block_size (b: Block): Z
+ := match block_fields b with
+    | nil => 2
+    | _ => 1 + Zlength (block_fields b)
+    end.
+
+Lemma block_size__eq (b: Block):
+    block_size b = Z.max 2 (1 + Zlength (block_fields b)).
+Proof.
+    unfold block_size.
+    remember (block_fields b) as ff eqn:Eff.
+    destruct ff as [|f ff] ; try easy.
+    pose proof (sublist.Zlength_nonneg ff) as H1.
+    rewrite Zlength_cons.
+    lia.
+Qed.
+
+Lemma block_size__lower_bound (b: Block):
+    2 <= block_size b.
+Proof.
+    rewrite block_size__eq.
+    lia.
+Qed.
+
+Lemma block_size__block_fields (b: Block):
+    1 + Zlength (block_fields b) <= block_size b <= 2 + Zlength (block_fields b).
+Proof.
+    rewrite block_size__eq.
+    remember (block_fields b) as ff eqn:Eff.
+    pose proof (sublist.Zlength_nonneg ff).
+    lia.
+Qed.
