theories/Block/vst/spec/spec.v
@@ -1,13 +1,93 @@
 From VST Require Import floyd.proofauto.
 
+From appliedfm Require Import int_or_ptr.vst.cmodel.val.
+
 From CertiCoq Require Import Block.vst.ast.ast.
+From CertiCoq Require Import Block.vst.cmodel.certicoq_block_header.
 From CertiCoq Require Import Block.vst.cmodel.certicoq_block.
 From CertiCoq Require Import Block.vst.clightgen.block.
 
+Definition theader: type
+ := if Archi.ptr64
+    then tulong
+    else tuint.
+
+Definition tsize_t: type
+ := if Archi.ptr64
+    then tulong
+    else tuint.
+
+Definition certicoq_block__get_size_spec :=
+  DECLARE _certicoq_block__get_size
+  WITH
+    h : BlockHeader,
+    sh : share,
+    p : val
+  PRE [ tptr theader ]
+    PROP (readable_share sh)
+    PARAMS (p)
+    GLOBALS ()
+    SEP (data_at sh (tarray theader 1) [block_header_encode_val h] p)
+  POST [ tsize_t ]
+    PROP ()
+    LOCAL (temp ret_temp (block_header_size_val h))
+    SEP (data_at sh (tarray theader 1) [block_header_encode_val h] p).
 
 
-(* 
+Definition certicoq_block__get_field_count_spec :=
+  DECLARE _certicoq_block__get_field_count
+  WITH
+    h : BlockHeader,
+    sh : share,
+    p : val
+  PRE [ tptr theader ]
+    PROP (readable_share sh)
+    PARAMS (p)
+    GLOBALS ()
+    SEP (data_at sh (tarray theader 1) [block_header_encode_val h] p)
+  POST [ tsize_t ]
+    PROP ()
+    LOCAL (temp ret_temp (block_header_field_count_val h))
+    SEP (data_at sh (tarray theader 1) [block_header_encode_val h] p).
+
+
+Definition certicoq_block__get_tag_spec :=
+  DECLARE _certicoq_block__get_tag
+  WITH
+    h : BlockHeader,
+    sh : share,
+    p : val
+  PRE [ tptr theader ]
+    PROP (readable_share sh)
+    PARAMS (p)
+    GLOBALS ()
+    SEP (data_at sh (tarray theader 1) [block_header_encode_val h] p)
+  POST [ tuchar ]
+    PROP ()
+    LOCAL (temp ret_temp (block_header_tag_val h))
+    SEP (data_at sh (tarray theader 1) [block_header_encode_val h] p).
+
+
+Definition certicoq_block__get_odata_spec :=
+  DECLARE _certicoq_block__get_odata
+  WITH
+    h : BlockHeader,
+    sh : share,
+    p : val
+  PRE [ tptr theader ]
+    PROP (readable_share sh)
+    PARAMS (p)
+    GLOBALS ()
+    SEP (data_at sh (tarray theader 1) [block_header_encode_val h] p)
+  POST [ tuchar ]
+    PROP ()
+    LOCAL (temp ret_temp (block_header_odata_val h))
+    SEP (data_at sh (tarray theader 1) [block_header_encode_val h] p).
+
+
 Definition ASI: funspecs := ltac:(with_library prog
-  [ (* TODO *)
+  [ certicoq_block__get_size_spec
+  ; certicoq_block__get_field_count_spec
+  ; certicoq_block__get_tag_spec
+  ; certicoq_block__get_odata_spec
   ]).
-*)
