theories/Block/vst/cmodel/certicoq_block_header.v
@@ -1,0 +1,223 @@
+From Coq Require Import micromega.Lia.
+From Coq Require Import ZArith.ZArith.
+
+From compcert Require Import common.Values.
+From compcert Require Import lib.Integers.
+
+From appliedfm Require Import int_or_ptr.vst.cmodel.constants.
+From appliedfm Require Import int_or_ptr.vst.cmodel.val.
+
+Local Open Scope Z.
+
+Record BlockHeader :=
+{
+  block_header_field_count: Z;
+  block_header_tag: Z;
+  block_header_odata: Z;
+  block_header_field_count__range: 0 <= block_header_field_count < two_p (word_size * 8 - 10);
+  block_header_tag__range: 0 <= block_header_tag < 256;
+  block_header_odata__range: 0 <= block_header_odata < 4;
+}.
+
+Lemma block_header_field_count__max (h: BlockHeader):
+  0 <= block_header_field_count h <= if Archi.ptr64 then Int64.max_unsigned else Int.max_unsigned.
+Proof.
+  admit.
+Admitted.
+
+
+Lemma block_header_tag__Int_max_unsigned (h: BlockHeader):
+  0 <= block_header_tag h <= Int.max_unsigned.
+Proof.
+  admit.
+Admitted.
+
+Lemma block_header_tag__Int64_max_unsigned (h: BlockHeader):
+  0 <= block_header_tag h <= Int64.max_unsigned.
+Proof.
+  pose proof (block_header_tag__Int_max_unsigned h) as HH1.
+  split ; try lia.
+  transitivity Int.max_unsigned ; try lia.
+  intro F.
+  inversion F.
+Qed.
+
+
+Lemma block_header_odata__max_unsigned (h: BlockHeader):
+  0 <= block_header_odata h <= Int.max_unsigned.
+Proof.
+  admit.
+Admitted.
+
+
+Definition block_header_field_count_val (h: BlockHeader): val
+ := if Archi.ptr64
+    then Vlong (Int64.repr (block_header_field_count h))
+    else Vint (Int.repr (block_header_field_count h)).
+
+Definition block_header_tag_val (h: BlockHeader): val
+ := Vint (Int.repr (block_header_tag h)).
+
+Definition block_header_odata_val (h: BlockHeader): val
+ := Vint (Int.repr (block_header_odata h)).
+
+Definition block_header_size (h: BlockHeader): Z
+ := Z.max 2 (1 + block_header_field_count h).
+
+
+Definition block_header_size_val (h: BlockHeader): val
+ := if Archi.ptr64
+    then Vlong (Int64.repr (block_header_size h))
+    else Vint (Int.repr (block_header_size h)).
+
+
+Definition block_header_field_count_encode (h: BlockHeader): Z
+ := Z.shiftl (block_header_field_count h) 10.
+
+
+Definition block_header_tag_encode (h: BlockHeader): Z
+ := block_header_tag h.
+
+
+Definition block_header_encode (h: BlockHeader): Z
+ := Z.lor
+      (Z.lor (block_header_field_count_encode h) (block_header_tag_encode h))
+      (Z.shiftl (block_header_odata h) 8).
+
+
+Lemma block_header_encode__max_unsigned (h: BlockHeader):
+  0 <= block_header_encode h <= if Archi.ptr64 then Int64.max_unsigned else Int.max_unsigned.
+Proof.
+  admit.
+Admitted.
+
+
+Definition block_header_encode_val (h: BlockHeader): val
+ := if Archi.ptr64
+    then Vlong (Int64.repr (block_header_encode h))
+    else Vint (Int.repr (block_header_encode h)).
+
+
+
+Lemma block_header_tag_encode__shiftr (h: BlockHeader) (x: Z) (Hx: 0 <= x):
+  Z.shiftr (block_header_tag_encode h) (8 + x) = 0.
+Proof.
+  rewrite <- Z.shiftr_shiftr by easy.
+  replace
+    (Z.shiftr (block_header_tag_encode h) 8)
+    with 0.
+  2: {
+    unfold block_header_tag_encode.
+    pose proof (block_header_tag__range h) as H1.
+    remember (block_header_tag h) as z eqn:Ez.
+    clear -H1.
+    destruct z ; try lia ; try easy.
+    do 9 (destruct p ; try easy).
+  }
+  apply Z.shiftr_0_l.
+Qed.
+
+Lemma block_header_encode__block_header_field_count (h: BlockHeader):
+  Z.shiftr (block_header_encode h) 10 = block_header_field_count h.
+Proof.
+  unfold block_header_encode.
+  repeat rewrite Z.shiftr_lor.
+  rewrite Z.shiftr_shiftl_l by lia.
+  replace (8-10) with (-2) by lia.
+  replace
+    (Z.shiftl (block_header_odata h) (-2))
+    with 0.
+  2: {
+    pose proof (block_header_odata__range h) as H1.
+    remember (block_header_odata h) as z eqn:Ez.
+    clear -H1.
+    destruct z ; try lia ; try easy.
+    do 3 (destruct p ; try easy).
+  }
+  rewrite Z.lor_0_r.
+  replace
+    (Z.shiftr (block_header_tag_encode h) 10)
+    with 0.
+  2: {
+    replace 10 with (8 + 2) by lia.
+    symmetry.
+    apply block_header_tag_encode__shiftr.
+    lia.
+  }
+  rewrite Z.lor_0_r.
+  unfold block_header_field_count_encode.
+  rewrite Z.shiftr_shiftl_l by lia.
+  now replace (10 - 10) with 0 by lia.
+Qed.
+
+
+Lemma block_header_encode__block_header_tag (h: BlockHeader):
+  Z.land (block_header_encode h) 255 = block_header_tag h.
+Proof.
+  unfold block_header_encode.
+  rewrite Z.land_lor_distr_l.
+  replace
+    (Z.land (Z.shiftl (block_header_odata h) 8) 255)
+    with 0.
+  2: {
+    pose proof (block_header_odata__range h) as H1.
+    remember (block_header_odata h) as z eqn:Ez.
+    clear -H1.
+    destruct z ; try lia ; try easy.
+  }
+  rewrite Z.lor_0_r.
+  rewrite Z.land_lor_distr_l.
+  replace
+    (Z.land (block_header_field_count_encode h) 255)
+    with 0.
+  2: {
+    unfold block_header_field_count_encode.
+    remember (block_header_field_count h) as z eqn:Ez.
+    clear.
+    destruct z ; try lia ; try easy.
+  }
+  rewrite Z.lor_0_l.
+  unfold block_header_tag_encode.
+  pose proof (block_header_tag__range h).
+  remember (block_header_tag h) as z eqn:Ez.
+  destruct z ; try lia ; try easy.
+  do 9 (destruct p ; try easy).
+Qed.
+
+
+Lemma block_header_encode__block_header_odata (h: BlockHeader):
+  Z.land (Z.shiftr (block_header_encode h) 8) 3 = block_header_odata h.
+Proof.
+  unfold block_header_encode.
+  repeat rewrite Z.shiftr_lor.
+  replace
+    (Z.shiftr (block_header_tag_encode h) 8)
+    with 0.
+  2: {
+    replace 8 with (8 + 0) by lia.
+    symmetry.
+    apply block_header_tag_encode__shiftr.
+    lia.
+  }
+  rewrite Z.lor_0_r.
+  rewrite Z.land_lor_distr_l.
+  replace
+    (Z.land (Z.shiftr (block_header_field_count_encode h) 8) 3)
+    with 0.
+  2: {
+    unfold block_header_field_count_encode.
+    rewrite Z.shiftr_shiftl_l by lia.
+    replace (10 - 8) with 2 by lia.
+    pose proof (block_header_field_count__range h).
+    remember (block_header_field_count h) as z eqn:Ez.
+    now destruct z.
+  }
+  rewrite Z.lor_0_l.
+  rewrite Z.shiftr_shiftl_l by lia.
+  replace (8 - 8) with 0 by lia.
+  pose proof (block_header_odata__range h) as H1.
+  remember (block_header_odata h) as z eqn:Ez.
+  clear -H1.
+  destruct z ; try lia ; try easy.
+  do 3 (destruct p ; try easy).
+Qed.
