theories/Block/vst/verif/certicoq_block__get_field_count.v
@@ -1,0 +1,21 @@
+From VST Require Import floyd.proofauto.
+
+From CertiCoq Require Import Block.vst.ast.ast.
+From CertiCoq Require Import Block.vst.clightgen.block.
+From CertiCoq Require Import Block.vst.cmodel.certicoq_block_header.
+From CertiCoq Require Import Block.vst.cmodel.certicoq_block.
+From CertiCoq Require Import Block.vst.spec.spec.
+
+Lemma body: semax_body Vprog ASI f_certicoq_block__get_field_count certicoq_block__get_field_count_spec.
+Proof.
+  start_function.
+  forward.
+  forward.
+  entailer!.
+  unfold block_header_field_count_val.
+  cbv [Archi.ptr64].
+  rewrite <- block_header_encode__block_header_field_count.
+  unfold Int64.shru.
+  rewrite Int64.unsigned_repr by apply block_header_encode__max_unsigned.
+  now change (Int64.unsigned (Int64.repr 10)) with 10.
+Qed.
