theories/Block/vst/verif/certicoq_block__get_odata.v
@@ -1,0 +1,29 @@
+From VST Require Import floyd.proofauto.
+
+From CertiCoq Require Import Block.vst.ast.ast.
+From CertiCoq Require Import Block.vst.clightgen.block.
+From CertiCoq Require Import Block.vst.cmodel.certicoq_block_header.
+From CertiCoq Require Import Block.vst.cmodel.certicoq_block.
+From CertiCoq Require Import Block.vst.spec.spec.
+
+Lemma body: semax_body Vprog ASI f_certicoq_block__get_odata certicoq_block__get_odata_spec.
+Proof.
+  start_function.
+  forward.
+  forward.
+  entailer!.
+  unfold block_header_odata_val.
+  replace
+    (Int64.unsigned (Int64.and (Int64.shru (Int64.repr (block_header_encode h)) (Int64.repr 8)) (Int64.repr 3)))
+    with (Z.land (Z.shiftr (block_header_encode h) 8) 3).
+  2: {
+    admit.
+  }
+  rewrite block_header_encode__block_header_odata.
+  f_equal.
+  pose proof (block_header_odata__range h) as HH.
+  remember (block_header_odata h) as z eqn:Ez.
+  clear -HH.
+  destruct z ; try lia ; try easy.
+  do 3 (destruct p ; try easy).
+Admitted.
