theories/Block/vst/verif/certicoq_block__get_size.v
@@ -1,0 +1,56 @@
+From VST Require Import floyd.proofauto.
+
+From CertiCoq Require Import Block.vst.ast.ast.
+From CertiCoq Require Import Block.vst.clightgen.block.
+From CertiCoq Require Import Block.vst.cmodel.certicoq_block_header.
+From CertiCoq Require Import Block.vst.cmodel.certicoq_block.
+From CertiCoq Require Import Block.vst.spec.spec.
+
+Lemma body: semax_body Vprog ASI f_certicoq_block__get_size certicoq_block__get_size_spec.
+Proof.
+  start_function.
+  forward.
+  forward.
+  forward.
+  forward_call.
+  forward_if (
+    PROP ()
+    LOCAL (temp _t'2 (block_header_size_val h))
+    SEP (data_at sh (tarray theader 1) [block_header_encode_val h] p)
+  ).
+  {
+    forward.
+    entailer!.
+    unfold block_header_size_val.
+    cbv [Archi.ptr64].
+    unfold block_header_size.
+    f_equal.
+    f_equal.
+    rewrite Int64.unsigned_repr in H.
+    2: {
+      split ; try lia.
+      intro F.
+      inversion F.
+    }
+    rewrite Int64.unsigned_repr in H by apply block_header_field_count__max.
+    lia.
+  }
+  {
+    forward.
+    entailer!.
+    unfold block_header_size_val.
+    cbv [Archi.ptr64].
+    unfold block_header_size.
+    rewrite Int64.unsigned_repr in H.
+    2: {
+      split ; try lia.
+      intro F.
+      inversion F.
+    }
+    rewrite Int64.unsigned_repr in H by apply block_header_field_count__max.
+    f_equal.
+    f_equal.
+    lia.
+  }
+  forward.
+Qed.
