theories/Block/vst/verif/certicoq_block__get_tag.v
@@ -1,0 +1,27 @@
+From VST Require Import floyd.proofauto.
+
+From CertiCoq Require Import Block.vst.ast.ast.
+From CertiCoq Require Import Block.vst.clightgen.block.
+From CertiCoq Require Import Block.vst.cmodel.certicoq_block_header.
+From CertiCoq Require Import Block.vst.cmodel.certicoq_block.
+From CertiCoq Require Import Block.vst.spec.spec.
+
+Lemma body: semax_body Vprog ASI f_certicoq_block__get_tag certicoq_block__get_tag_spec.
+Proof.
+  start_function.
+  forward.
+  forward.
+  entailer!.
+  unfold block_header_tag_val.
+  rewrite block_header_encode__block_header_tag.
+  rewrite Int64.unsigned_repr by apply block_header_tag__Int64_max_unsigned.
+  unfold Int.zero_ext.
+  rewrite Int.unsigned_repr by apply block_header_tag__Int_max_unsigned.
+  f_equal.
+  f_equal.
+  pose proof (block_header_tag__range h) as HH.
+  remember (block_header_tag h) as z eqn:Ez.
+  clear -HH.
+  destruct z ; try lia ; try easy.
+  do 9 (destruct p ; try easy).
+Qed.
