theories/Block/vst/verif/verif.v
@@ -1,6 +1,0 @@
-From VST Require Import floyd.proofauto.
-
-From CertiCoq Require Import Block.vst.ast.ast.
-From CertiCoq Require Import Block.vst.clightgen.block.
-From CertiCoq Require Import Block.vst.cmodel.certicoq_block.
-From CertiCoq Require Import Block.vst.spec.spec.
